theories/Dot/path_wp.v
@@ -1,6 +1,6 @@
 From iris.proofmode Require Import tactics.
 From D Require Import iris_prelude.
-From D.Dot Require Import operational synLemmas.
+From D.Dot Require Import operational synLemmas rules.
 
 Implicit Types
          (L T U: ty) (v: vl) (e: tm) (d: dm) (ds: dms) (p : path)
@@ -129,5 +129,49 @@ Section path_wp.
       iDestruct "H" as (? Hl) "> ->". iIntros "!%" (Hclps).
       enough (nclosed (dvl v) n). by eauto with fv.
       eapply nclosed_lookup', Himpl; eauto with fv.
+  Qed.
+
+  Lemma path_wp_timeless_len φ p:
+    (∀ v, Timeless (φ v)) →
+    path_wp p φ ⊢ ▷^(plength p) False ∨ ∃ v, path_wp p (λ w, ⌜ w = v ⌝) ∧ φ v.
+  Proof.
+    rewrite path_wp_eq. intros Htime. iDestruct 1 as (v) "(Heq & Hv)".
+    iDestruct (timeless_timelessN with "Hv") as "[H | H]"; eauto.
+  Qed.
+
+  Fixpoint path2tm p: tm :=
+    match p with
+    | pv v => tv v
+    | pself p l => tproj (path2tm p) l
+    end.
+
+  (* Until stdpp upgrade; upstreamed in
+     https://gitlab.mpi-sws.org/iris/stdpp/merge_requests/87
+   *)
+  Fail Check nsteps_once_inv.
+  Lemma nsteps_once_inv `(R : relation A) x y :
+    relations.nsteps R 1 x y → R x y.
+  Proof. inversion 1 as [|???? Hhead Htail]; inversion Htail; by subst. Qed.
+
+  Lemma path_wp_exec p v :
+    path_wp p (λ w, ⌜ w = v ⌝) ⊢ ▷^(plength p) ⌜ PureExec True (plength p) (path2tm p) (tv v) ⌝.
+  Proof.
+    iInduction p as [w|] "IHp" forall (v); rewrite /PureExec/=.
+    - iIntros (-> _). by iIntros "!%"; constructor.
+    - iIntros "#Hp" (_). iDestruct (path_wp_eq with "Hp") as (vp) "{Hp}(Hp&Hs)".
+      iSpecialize ("IHp" with "Hp"). iClear "Hp".
+      rewrite -swap_later. iNext (plength p).
+      iDestruct "IHp" as %Hpure. iDestruct "Hs" as (vq Hlook) "> ->".
+      iIntros "!%". eapply nsteps_r.
+      + by apply (pure_step_nsteps_ctx (fill_item (ProjCtx l))), Hpure.
+      + apply nsteps_once_inv, pure_tproj, Hlook.
+  Qed.
+
+  Lemma path_wp_adequacy p φ :
+    (∀ v, Timeless (φ v)) →
+    path_wp p φ ⊢ ▷^(plength p) False ∨ (∃ v, ⌜ PureExec True (plength p) (path2tm p) (tv v) ⌝ ∧ φ v).
+  Proof.
+    intros Htime. rewrite path_wp_timeless_len; iDestruct 1 as "[$|H]".
+    iApply timeless_timelessN. setoid_rewrite path_wp_exec. iNext. eauto.
   Qed.
 End path_wp.
